checkpoint before some more updates of mem-simulation.
NOTE: found an inconsistent between this proof and the old proofs. The
old proofs assume that malloc zeros-out all metadata indiced by the
address in the allocation range. Otherwise, if malloc reuses free-ed
addresses that have old metadata, then runtime can load wrong metadata
for the reused address.

The SoftBound implementation for llvm-2.6 does not create wrappers for
malloc, so the above assumption (zero-out metadata) is not true. This is
because llvm 2.6 takes malloc as a primitive insn. SoftBound supports
malloc wrapper for llvm 2.7>=, which takes malloc as intrinsic
functions.

This is not a problem for the current memory model because it has
infinite memory, and does not reuse any deallocated address. But this
must be a problem to prove CETS for llvm 2.6 since we need a more
realistic memory model that reuses memory.



git-svn-id: https://webdav.seas.upenn.edu/svn/sol/vol@2881 eef5ea85-cc2e-0410-bd84-0fae1f012da8

src/SoftBound/sb_trans.v
@@ -613,55 +613,94 @@ end.
 
 (* Simulation *)
 
-Definition reg_simulation (rm1:SoftBound.rmetadata) (rm2:rmap) (lc1 lc2:GVMap) 
-  : Prop :=
-(forall i0 gv, lookupAL _ lc1 i0 = Some gv -> lookupAL _ lc2 i0 = Some gv) /\
-(forall pid bgv egv, 
-  lookupAL _ rm1 pid = Some (SoftBound.mkMD bgv egv) -> 
-  exists bid, exists eid, 
-    lookupAL _ rm2 pid = Some (bid, eid) /\
-    lookupAL _ lc2 bid = Some bgv /\
-    lookupAL _ lc2 eid = Some egv) /\
-(forall pid bid eid bgv egv, 
-  lookupAL _ rm2 pid = Some (bid, eid) ->
-  lookupAL _ lc2 bid = Some bgv ->
-  lookupAL _ lc2 eid = Some egv ->
-  lookupAL _ rm1 pid = Some (SoftBound.mkMD bgv egv)).
+Definition gv_inject (mi: Values.meminj) (gv gv':GenericValue) : Prop :=
+let '(vals,mks) := List.split gv in 
+let '(vals',mks') := List.split gv' in 
+val_list_inject mi vals vals' /\ mks = mks'.
 
-Definition sb_meminj (b:Values.block) : option (Values.block * Z) :=
-  Some (b, 0%Z).
-
-Definition sb_mem_inj (M M':mem) := Memory.Mem.mem_inj sb_meminj M M'.
-
-Definition mem_simulation TD (MM1:SoftBound.mmetadata) (Mem1 Mem2:mem) : Prop :=
-sb_mem_inj Mem1 Mem2 /\
-(forall lc gl b i bgv egv als lc' Mem2' tr addrb addre bid0 eid0 als' v, 
-  MM1 b i = Some (SoftBound.mkMD bgv egv) ->
-  getOperandValue TD Mem1 v lc gl = Some (ptr2GV TD (Vptr b i)) ->
-  SimpleSE.dbCmds TD gl lc als Mem2
-    (insn_call fake_id true false typ_void get_mmetadata_fn 
-       ((p8,v)::
-        (p8,(value_id addrb))::
-        (p8,(value_id addre))::nil)::
-     insn_load bid0 p8 (value_id addrb) Align.Zero::
-     insn_load eid0 p8 (value_id addre) Align.Zero::   
-     nil) lc' als' Mem2' tr ->
-  lookupAL _ lc' bid0 = Some bgv /\
-  lookupAL _ lc' bid0 = Some egv
+Definition reg_simulation (mi:Values.meminj) (rm1:SoftBound.rmetadata) 
+  (rm2:rmap) (lc1 lc2:GVMap) : Prop :=
+(forall i0 gv1, 
+  lookupAL _ lc1 i0 = Some gv1 -> 
+  exists gv2, 
+    lookupAL _ lc2 i0 = Some gv2 /\ gv_inject mi gv1 gv2
 ) /\
-(forall lc gl b i bgv egv als lc' Mem2' tr addrb addre bid0 eid0 als' v, 
-  getOperandValue TD Mem1 v lc gl = Some (ptr2GV TD (Vptr b i)) ->
-  SimpleSE.dbCmds TD gl lc als Mem2
+(forall pid bgv1 egv1, 
+  lookupAL _ rm1 pid = Some (SoftBound.mkMD bgv1 egv1) -> 
+  exists bid, exists eid, exists bgv2, exists egv2,
+    lookupAL _ rm2 pid = Some (bid, eid) /\
+    lookupAL _ lc2 bid = Some bgv2 /\
+    lookupAL _ lc2 eid = Some egv2 /\
+    gv_inject mi bgv1 bgv2 /\
+    gv_inject mi egv1 egv2
+) /\
+(forall pid bid eid bgv2 egv2, 
+  lookupAL _ rm2 pid = Some (bid, eid) ->
+  lookupAL _ lc2 bid = Some bgv2 ->
+  lookupAL _ lc2 eid = Some egv2 ->
+  exists bgv1, exists egv1,
+    lookupAL _ rm1 pid = Some (SoftBound.mkMD bgv1 egv1) /\
+    gv_inject mi bgv1 bgv2 /\
+    gv_inject mi egv1 egv2
+).
+
+Definition mem_simulation (mi:Values.meminj) TD (MM1:SoftBound.mmetadata) 
+  (Mem1 Mem2:mem) : Prop :=
+Mem.mem_inj mi Mem1 Mem2 /\
+(forall lc2 gl b1 i1 bgv egv als addrb addre bid0 eid0 v b2 i2,  
+  MM1 b1 i1 = Some (SoftBound.mkMD bgv egv) ->
+  Values.val_inject mi (Vptr b1 i1) (Vptr b2 i2) ->
+  getOperandValue TD Mem2 v lc2 gl = Some (ptr2GV TD (Vptr b2 i2)) ->
+  exists bgv', exists egv', exists lc2', exists Mem2',
+  SimpleSE.dbCmds TD gl lc2 als Mem2
     (insn_call fake_id true false typ_void get_mmetadata_fn 
        ((p8,v)::
         (p8,(value_id addrb))::
         (p8,(value_id addre))::nil)::
      insn_load bid0 p8 (value_id addrb) Align.Zero::
      insn_load eid0 p8 (value_id addre) Align.Zero::   
-     nil) lc' als' Mem2' tr ->
-  lookupAL _ lc' bid0 = Some bgv ->
-  lookupAL _ lc' bid0 = Some egv ->
-  MM1 b i = Some (SoftBound.mkMD bgv egv)
+     nil) lc2' als Mem2' trace_nil /\
+    lookupAL _ lc2' bid0 = Some bgv' /\
+    lookupAL _ lc2' eid0 = Some egv' /\
+    gv_inject mi bgv bgv' /\
+    gv_inject mi egv egv' /\
+    Mem.mem_inj mi Mem2 Mem2'
+) /\
+(forall lc2 gl b1 i1 als addrb addre bid0 eid0 v b2 i2,  
+  MM1 b1 i1 = None ->
+  Values.val_inject mi (Vptr b1 i1) (Vptr b2 i2) ->
+  getOperandValue TD Mem2 v lc2 gl = Some (ptr2GV TD (Vptr b2 i2)) ->
+  exists lc2', exists Mem2',
+  SimpleSE.dbCmds TD gl lc2 als Mem2
+    (insn_call fake_id true false typ_void get_mmetadata_fn 
+       ((p8,v)::
+        (p8,(value_id addrb))::
+        (p8,(value_id addre))::nil)::
+     insn_load bid0 p8 (value_id addrb) Align.Zero::
+     insn_load eid0 p8 (value_id addre) Align.Zero::   
+     nil) lc2' als Mem2' trace_nil /\
+    lookupAL _ lc2' bid0 = Some null /\
+    lookupAL _ lc2' eid0 = Some null /\
+    Mem.mem_inj mi Mem2 Mem2'
+) /\
+(forall gl b2 i2 bgv' egv' als lc2 lc2' addrb addre bid0 eid0 v Mem2', 
+  getOperandValue TD Mem2 v lc2 gl = Some (ptr2GV TD (Vptr b2 i2)) ->
+  SimpleSE.dbCmds TD gl lc2 als Mem2
+    (insn_call fake_id true false typ_void get_mmetadata_fn 
+       ((p8,v)::
+        (p8,(value_id addrb))::
+        (p8,(value_id addre))::nil)::
+     insn_load bid0 p8 (value_id addrb) Align.Zero::
+     insn_load eid0 p8 (value_id addre) Align.Zero::   
+     nil) lc2' als Mem2' trace_nil ->
+  lookupAL _ lc2' bid0 = Some bgv' ->
+  lookupAL _ lc2' eid0 = Some egv' ->
+  exists bgv, exists egv, exists b1, exists i1,
+    MM1 b1 i1 = Some (SoftBound.mkMD bgv egv) /\
+    Values.val_inject mi (Vptr b1 i1) (Vptr b2 i2) /\
+    gv_inject mi bgv bgv' /\
+    gv_inject mi egv egv' /\
+    Mem.mem_inj mi Mem2 Mem2'
 ).
 
 Fixpoint codom (rm:rmap) : atoms :=
@@ -689,34 +728,37 @@ Proof.
       auto.
 Qed.
 
-Lemma reg_simulation__updateAddAL : forall rm1 rm2 lc1 lc2 i0 gv',
-  reg_simulation rm1 rm2 lc1 lc2 ->
+Lemma reg_simulation__updateAddAL : forall mi rm1 rm2 lc1 lc2 i0 gv gv',
+  reg_simulation mi rm1 rm2 lc1 lc2 ->
   i0 `notin` codom rm2 ->
-  reg_simulation rm1 rm2 (updateAddAL GenericValue lc1 i0 gv')
+  gv_inject mi gv gv' ->
+  reg_simulation mi rm1 rm2 (updateAddAL GenericValue lc1 i0 gv)
     (updateAddAL GenericValue lc2 i0 gv').
 Proof.
-  intros rm1 rm2 lc1 lc2 i0 gv' Hsim Hnotin. 
+  intros mi rm1 rm2 lc1 lc2 i0 gv gv' Hsim Hnotin. 
   destruct Hsim as [J1 [J2 J3]].    
   split.
-    intros i1 gv J.
+    intros i1 gv1 J.
     destruct (id_dec i0 i1); subst.
       rewrite lookupAL_updateAddAL_eq in *; auto.
+      inv J.
+      exists gv'. auto.
     
       rewrite <- lookupAL_updateAddAL_neq in J; auto.
       rewrite <- lookupAL_updateAddAL_neq; auto.
   split.
-    intros pid bbgv egv J.
+    intros pid bgv1 egv1 J.
     apply J2 in J. 
-    destruct J as [bid [eid [J11 [J12 J13]]]].
-    exists bid. exists eid.
+    destruct J as [bid [eid [bgv2 [egv2 [J11 [J12 [J13 [J14 J15]]]]]]]].
+    exists bid. exists eid. exists bgv2. exists egv2.
+    assert (J11':=J11).
+    apply in_codom_of_rmap in J11'.    
+    destruct J11' as [J16 J17].      
+    rewrite <- lookupAL_updateAddAL_neq; try solve [fsetdec].
+    rewrite <- lookupAL_updateAddAL_neq; try solve [fsetdec].
     split; auto.
-      apply in_codom_of_rmap in J11.    
-      destruct J11 as [J11 J14].
-      
-      rewrite <- lookupAL_updateAddAL_neq; try solve [fsetdec].
-      rewrite <- lookupAL_updateAddAL_neq; try solve [fsetdec].
 
-    intros pid bid eid bgv egv H1 H2 H3.
+    intros pid bid eid bgv2 egv2 H1 H2 H3.
     assert (H1':=H1).
     apply in_codom_of_rmap in H1'.    
     destruct H1' as [H11 H12].
@@ -725,21 +767,155 @@ Proof.
     eauto.
 Qed.
 
+Lemma _zeroconst2GV__gv_inject_refl : forall TD t gv mi,
+  _zeroconst2GV TD t = Some gv ->
+  gv_inject mi gv gv.
+Admitted.
 
-Definition sb_mem_inj__const2GV_prop (c:const) := forall Mem1 Mem2 TD gl gv,
-  sb_mem_inj Mem1 Mem2 ->
-  _const2GV TD Mem1 gl c = Some gv ->
-  _const2GV TD Mem2 gl c = Some gv.
+Lemma gv_inject__eq__sizeGenericValue : forall mi gv1 gv2,
+  gv_inject mi gv1 gv2 ->
+  sizeGenericValue gv1 = sizeGenericValue gv2.
+Admitted.
+
+Lemma val_list_inject_app : forall mi vs1 vs1' vs2 vs2',
+  val_list_inject mi vs1 vs2 ->
+  val_list_inject mi vs1' vs2' ->
+  val_list_inject mi (vs1++vs1') (vs2++vs2').
+Admitted.
+
+Lemma gv_inject_app : forall mi gv1 gv1' gv2 gv2',
+  gv_inject mi gv1 gv2 ->
+  gv_inject mi gv1' gv2' ->
+  gv_inject mi (gv1++gv1') (gv2++gv2').
+Admitted.
+
+Lemma global_gv_inject_refl : forall mi gl i0 gv,
+  lookupAL _ gl i0 = Some gv ->
+  gv_inject mi gv gv.
+Admitted.
+    
+Lemma simulation__mtrunc : forall mi TD top t1 gv1 t2 gv1' gv2,
+  gv_inject mi gv1 gv1' ->
+  mtrunc TD top t1 gv1 t2 = Some gv2 ->
+  exists gv2',
+    mtrunc TD top t1 gv1' t2 = Some gv2' /\
+    gv_inject mi gv2 gv2'.
+Admitted.
+
+Lemma simulation__mext : forall mi TD eop t1 gv1 t2 gv1' gv2,
+  gv_inject mi gv1 gv1' ->
+  mext TD eop t1 gv1 t2 = Some gv2 ->
+  exists gv2',
+    mext TD eop t1 gv1' t2 = Some gv2' /\
+    gv_inject mi gv2 gv2'.
+Admitted.
+
+Lemma simulation__mbop : forall mi TD op bsz gv1 gv1' gv2 gv2' gv3,
+  gv_inject mi gv1 gv1' ->
+  gv_inject mi gv2 gv2' ->
+  mbop TD op bsz gv1 gv2 = Some gv3 ->
+  exists gv3',
+    mbop TD op bsz gv1' gv2' = Some gv3' /\
+    gv_inject mi gv3 gv3'.
+Admitted.
+
+Lemma simulation__mfbop : forall mi TD op fp gv1 gv1' gv2 gv2' gv3,
+  gv_inject mi gv1 gv1' ->
+  gv_inject mi gv2 gv2' ->
+  mfbop TD op fp gv1 gv2 = Some gv3 ->
+  exists gv3',
+    mfbop TD op fp gv1' gv2' = Some gv3' /\
+    gv_inject mi gv3 gv3'.
+Admitted.
+
+Lemma simulation__mcast : forall mi TD Mem1 Mem2 op t1 gv1 gv1' t2 gv2,
+  gv_inject mi gv1 gv1' ->
+  Mem.mem_inj mi Mem1 Mem2 ->  
+  mcast TD Mem1 op t1 gv1 t2 = Some gv2 ->
+  exists gv2',
+    mcast TD Mem2 op t1 gv1' t2 = Some gv2' /\
+    gv_inject mi gv2 gv2'.
+Admitted.
+
+Lemma simulation__micmp : forall mi TD c t gv1 gv1' gv2 gv2' gv3,
+  gv_inject mi gv1 gv1' ->
+  gv_inject mi gv2 gv2' ->
+  micmp TD c t gv1 gv2 = Some gv3 ->
+  exists gv3',
+    micmp TD c t gv1' gv2' = Some gv3' /\
+    gv_inject mi gv3 gv3'.
+Admitted.
+
+Lemma simulation__mfcmp : forall mi TD c t gv1 gv1' gv2 gv2' gv3,
+  gv_inject mi gv1 gv1' ->
+  gv_inject mi gv2 gv2' ->
+  mfcmp TD c t gv1 gv2 = Some gv3 ->
+  exists gv3',
+    mfcmp TD c t gv1' gv2' = Some gv3' /\
+    gv_inject mi gv3 gv3'.
+Admitted.
+
+Lemma simulation__GV2ptr : forall mi TD gv1 gv1' v,
+  gv_inject mi gv1 gv1' ->
+  GV2ptr TD (getPointerSize TD) gv1 = Some v ->
+  exists v',
+    GV2ptr TD (getPointerSize TD) gv1' = Some v' /\
+    Values.val_inject mi v v'.
+Admitted.
+
+Lemma simulation__mgep : forall mi TD v v' v0 t0 l1,
+  Values.val_inject mi v v' ->
+  mgep TD t0 v l1 = Some v0 ->
+  exists v0',
+    mgep TD t0 v' l1 = Some v0' /\
+    Values.val_inject mi v0 v0'.
+Admitted.
+   
+Lemma gv_inject__eq__isGVZero : forall mi TD gv gv',
+  gv_inject mi gv gv' ->
+  isGVZero TD gv = isGVZero TD gv'.
+Admitted.
+
+Lemma simulation__extractGenericValue : forall mi gv1 gv1' TD t1 l0 gv,
+  gv_inject mi gv1 gv1' ->
+  extractGenericValue TD t1 gv1 l0 = Some gv ->
+  exists gv',
+    extractGenericValue TD t1 gv1' l0 = Some gv' /\
+    gv_inject mi gv gv'.
+Admitted.
+
+Lemma simulation__insertGenericValue : forall mi gv1 gv1' TD t1 l0 gv t2 gv2 
+                                              gv2',
+  gv_inject mi gv1 gv1' ->
+  gv_inject mi gv2 gv2' ->
+  insertGenericValue TD t1 gv1 l0 t2 gv2 = Some gv ->
+  exists gv',
+    insertGenericValue TD t1 gv1' l0 t2 gv2' = Some gv' /\
+    gv_inject mi gv gv'.
+Admitted.
+
+Definition sb_mem_inj__const2GV_prop (c:const) := forall mi Mem1 Mem2 TD gl gv t,
+  Mem.mem_inj mi Mem1 Mem2 ->
+  _const2GV TD Mem1 gl c = Some (gv,t) ->
+  exists gv',
+    _const2GV TD Mem2 gl c = Some (gv',t) /\
+    gv_inject mi gv gv'.
 
 Definition sb_mem_inj__list_const2GV_prop (lc:list_const) := 
-  forall Mem1 Mem2 TD gl,
-  sb_mem_inj Mem1 Mem2 ->
-  (forall gv, 
-    _list_const_arr2GV TD Mem1 gl lc = Some gv ->
-    _list_const_arr2GV TD Mem2 gl lc = Some gv) /\
-  (forall R, 
-    _list_const_struct2GV TD Mem1 gl lc = Some R ->
-    _list_const_struct2GV TD Mem2 gl lc = Some R).
+  forall mi Mem1 Mem2 TD gl,
+  Mem.mem_inj mi Mem1 Mem2 ->
+  (forall gv t, 
+    _list_const_arr2GV TD Mem1 gl lc = Some (gv,t) ->
+    exists gv',
+      _list_const_arr2GV TD Mem2 gl lc = Some (gv',t) /\
+      gv_inject mi gv gv'
+  ) /\
+  (forall gv t a, 
+    _list_const_struct2GV TD Mem1 gl lc = Some (gv,t,a) ->
+    exists gv',
+      _list_const_struct2GV TD Mem2 gl lc = Some (gv',t,a) /\
+      gv_inject mi gv gv'
+  ).
 
 Lemma sb_mem_inj__const2GV_mutrec :
   (forall c, sb_mem_inj__const2GV_prop c) *
@@ -749,6 +925,38 @@ Proof.
     unfold sb_mem_inj__const2GV_prop, sb_mem_inj__list_const2GV_prop;
     intros; simpl in *; eauto.
 
+  remember (_zeroconst2GV TD t) as R.
+  destruct R; inv H0.
+  exists gv. split; eauto using _zeroconst2GV__gv_inject_refl.
+
+  inv H0.
+  exists (val2GV TD
+            (Vint (Size.to_nat s - 1)
+               (Int.repr (Size.to_nat s - 1) (INTEGER.to_Z i0)))
+            (AST.Mint (Size.to_nat s - 1))).
+  split; try solve [auto | unfold val2GV, gv_inject; simpl; auto].
+
+  destruct f; inv H0.
+    exists (val2GV TD (Vfloat f0) AST.Mfloat32).
+    split; try solve [auto | unfold val2GV, gv_inject; simpl; auto].
+
+    exists (val2GV TD (Vfloat f0) AST.Mfloat64).
+    split; try solve [auto | unfold val2GV, gv_inject; simpl; auto].
+
+  remember (getTypeSizeInBits TD t) as R.
+  destruct R; inv H0.
+  exists (val2GV TD Vundef (AST.Mint (n - 1))).
+  split; try solve [auto | unfold val2GV, gv_inject; simpl; auto].
+  
+  inv H0.
+  exists (val2GV TD (Vptr Mem.nullptr (Int.repr 31 0)) (AST.Mint 31)).
+  split; auto. 
+    unfold val2GV, gv_inject; simpl.
+    split; auto.
+      apply val_cons_inject; auto.
+      apply val_inject_ptr with (delta:=0); auto.
+      admit. (* mi should map null to null. *)
+ 
   apply H with (TD:=TD)(gl:=gl) in H0.
   destruct H0; eauto.
 
@@ -756,93 +964,250 @@ Proof.
   destruct H0 as [H00 H01].
   remember (_list_const_struct2GV TD Mem1 gl l0) as R.
   destruct R as [[[gv1 t1] a1]|]; inv H1.
-  erewrite H01; eauto.
-  simpl. auto.
+  destruct (@H01 gv1 t1 a1) as [gv' [H02 H03]]; auto.
+  rewrite H02; auto.
+  erewrite <- gv_inject__eq__sizeGenericValue; eauto.
+  remember (sizeGenericValue gv1) as R1.
+  destruct R1; inv H2.
+    exists (uninits (Align.to_nat a1)).
+    split; auto.
+      unfold uninits, gv_inject; simpl; auto.
+
+    exists (gv' ++ uninits (Align.to_nat a1 - S R1)).
+    split; auto.
+      unfold uninits.
+      apply gv_inject_app; auto.
+        unfold gv_inject; simpl; auto.       
+
+  remember (lookupAL GenericValue gl i0) as R.
+  destruct R; inv H0.
+  exists gv. split; eauto using global_gv_inject_refl.
 
   remember (_const2GV TD Mem1 gl c) as R.
-  destruct R as [[gv1 t1]|]; inv H1.
-  erewrite H; eauto.
-  simpl; auto.
+  destruct R as [[gv1 t1']|]; inv H1.
+  symmetry in HeqR.
+  eapply H in HeqR; eauto.
+  destruct HeqR as [gv' [J1 J2]].
+  rewrite J1.
+  remember (mtrunc TD t t1' gv1 t0) as R1.
+  destruct R1; inv H3.
+  symmetry in HeqR1.
+  eapply simulation__mtrunc in HeqR1; eauto.
+  destruct HeqR1 as [gv2' [J3 J4]].
+  rewrite J3.
+  exists gv2'. split; auto.
 
   remember (_const2GV TD Mem1 gl c) as R.
-  destruct R as [[gv1 t1]|]; inv H1.
-  erewrite H; eauto.
-  simpl; auto.
+  destruct R as [[gv1 t1']|]; inv H1.
+  symmetry in HeqR.
+  eapply H in HeqR; eauto.
+  destruct HeqR as [gv' [J1 J2]].
+  rewrite J1.
+  remember (mext TD e t1' gv1 t) as R1.
+  destruct R1; inv H3.
+  symmetry in HeqR1.
+  eapply simulation__mext in HeqR1; eauto.
+  destruct HeqR1 as [gv2' [J3 J4]].
+  rewrite J3.
+  exists gv2'. split; auto.
 
-      remember (_const2GV TD Mem1 gl c0) as R.
-      destruct R as [[gv1 t1]|]; inv H1.
-      erewrite H; eauto.
-      simpl.
-      admit.
+  remember (_const2GV TD Mem1 gl c0) as R.
+  destruct R as [[gv1 t1']|]; inv H1.
+  symmetry in HeqR.
+  eapply H in HeqR; eauto.
+  destruct HeqR as [gv' [J1 J2]].
+  rewrite J1.
+  remember (mcast TD Mem1 c t1' gv1 t) as R1.
+  destruct R1; inv H3.
+  symmetry in HeqR1.
+  eapply simulation__mcast in HeqR1; eauto.
+  destruct HeqR1 as [gv2' [J3 J4]].
+  rewrite J3.
+  exists gv2'. split; auto.
 
-      remember (Constant.getTyp c) as R.
-      destruct R; inv H2.       
-      destruct t; inv H4.       
-      remember (_const2GV TD Mem1 gl c) as R1.
-      destruct R1 as [[gv1 t1]|]; inv H3.
-      erewrite H; eauto.
-      simpl. auto.
+  remember (Constant.getTyp c) as R.
+  destruct R; inv H2.       
+  destruct t0; inv H4.       
+  remember (_const2GV TD Mem1 gl c) as R1.
+  destruct R1 as [[gv1 t1]|]; inv H3.
+  remember (getConstGEPTyp l0 t0) as R2.
+  destruct R2; inv H4.
+  remember (GV2ptr TD (getPointerSize TD) gv1) as R3.
+  destruct R3; inv H3.
+  remember (intConsts2Nats TD l0) as R4.
+  destruct R4; inv H4.
+  remember (mgep TD t0 v l1) as R5.
+  destruct R5; inv H3.
+  symmetry in HeqR1.
+  eapply H in HeqR1; eauto.
+  destruct HeqR1 as [gv1' [J1 J2]].
+  rewrite J1.
+  symmetry in HeqR3.
+  eapply simulation__GV2ptr in HeqR3; eauto.
+  destruct HeqR3 as [v' [J3 J4]].
+  rewrite J3.  
+  symmetry in HeqR5.
+  eapply simulation__mgep in HeqR5; eauto.
+  destruct HeqR5 as [v0' [J5 J6]].
+  rewrite J5.
+  exists (ptr2GV TD v0').
+  split; auto.
+    unfold ptr2GV, val2GV, gv_inject. simpl. auto.
 
-      remember (_const2GV TD Mem1 gl c) as R2.
-      destruct R2 as [[gv2 t2]|]; inv H3.
-      remember (_const2GV TD Mem1 gl c0) as R3.
-      destruct R3 as [[gv3 t3]|]; inv H5.
-      remember (_const2GV TD Mem1 gl c2) as R4.
-      destruct R4 as [[gv4 t4]|]; inv H4.
-      erewrite H; eauto.
-      erewrite H0; eauto.
-      erewrite H1; eauto.
+  remember (_const2GV TD Mem1 gl c) as R2.
+  destruct R2 as [[gv2 t2]|]; inv H3.
+  remember (_const2GV TD Mem1 gl c0) as R3.
+  destruct R3 as [[gv3 t3]|]; inv H5.
+  remember (_const2GV TD Mem1 gl c2) as R4.
+  destruct R4 as [[gv4 t4]|]; inv H4.
+  symmetry in HeqR2. 
+  eapply H in HeqR2; eauto.
+  destruct HeqR2 as [gv2' [J1 J2]].
+  rewrite J1.
+  symmetry in HeqR3. 
+  eapply H0 in HeqR3; eauto.
+  destruct HeqR3 as [gv3' [J3 J4]].
+  rewrite J3.
+  symmetry in HeqR4. 
+  eapply H1 in HeqR4; eauto.
+  destruct HeqR4 as [gv4' [J5 J6]].
+  rewrite J5.
+  erewrite <- gv_inject__eq__isGVZero; eauto.
+  destruct (isGVZero TD gv2); inv H5.
+    exists gv4'. split; auto.
+    exists gv3'. split; auto.
 
-      remember (_const2GV TD Mem1 gl c0) as R3.
-      destruct R3 as [[gv3 t3]|]; inv H2.
-      remember (_const2GV TD Mem1 gl c2) as R4.
-      destruct R4 as [[gv4 t4]|]; inv H4.
-      erewrite H; eauto.
-      erewrite H0; eauto.
-      simpl. auto.
+  remember (_const2GV TD Mem1 gl c0) as R3.
+  destruct R3 as [[gv3 t3]|]; inv H2.
+  remember (_const2GV TD Mem1 gl c2) as R4.
+  destruct R4 as [[gv4 t4]|]; inv H4.
+  symmetry in HeqR3. 
+  eapply H in HeqR3; eauto.
+  destruct HeqR3 as [gv3' [J3 J4]].
+  rewrite J3.
+  symmetry in HeqR4. 
+  eapply H0 in HeqR4; eauto.
+  destruct HeqR4 as [gv4' [J5 J6]].
+  rewrite J5.
+  remember (micmp TD c t3 gv3 gv4) as R1.
+  destruct R1; inv H3.
+  symmetry in HeqR1.
+  eapply simulation__micmp in HeqR1; eauto.
+  destruct HeqR1 as [gv' [J7 J8]].
+  rewrite J7.
+  exists gv'. split; auto.
 
-      remember (_const2GV TD Mem1 gl c) as R3.
-      destruct R3 as [[gv3 t3]|]; inv H2.
-      remember (_const2GV TD Mem1 gl c0) as R4.
-      destruct R4 as [[gv4 t4]|]; inv H4.
-        erewrite H; eauto.
-        erewrite H0; eauto.
-        simpl. auto.
-
-        destruct t3; inv H3.
-      
+  remember (_const2GV TD Mem1 gl c) as R3.
+  destruct R3 as [[gv3 t3]|]; inv H2.
+  destruct t3; inv H4.
+  remember (_const2GV TD Mem1 gl c0) as R4.
+  destruct R4 as [[gv4 t4]|]; inv H3.
+  symmetry in HeqR3. 
+  eapply H in HeqR3; eauto.
+  destruct HeqR3 as [gv3' [J3 J4]].
+  rewrite J3.
+  symmetry in HeqR4. 
+  eapply H0 in HeqR4; eauto.
+  destruct HeqR4 as [gv4' [J5 J6]].
+  rewrite J5.
+  remember (mfcmp TD f f0 gv3 gv4) as R1.
+  destruct R1; inv H4.
+  symmetry in HeqR1.
+  eapply simulation__mfcmp in HeqR1; eauto.
+  destruct HeqR1 as [gv' [J7 J8]].
+  rewrite J7.
+  exists gv'. split; auto.
+     
   remember (_const2GV TD Mem1 gl c) as R.
   destruct R as [[gv1 t1]|]; inv H2.
-  erewrite H; eauto.
-  simpl; auto.
+  remember (Constant.getTyp c) as R1.
+  destruct R1; inv H4.       
+  remember (getSubTypFromConstIdxs l0 t0) as R2.
+  destruct R2; inv H3.   
+  remember (extractGenericValue TD t1 gv1 l0) as R3.
+  destruct R3; inv H4.   
+  symmetry in HeqR. 
+  eapply H in HeqR; eauto.
+  destruct HeqR as [gv1' [J1 J2]].
+  rewrite J1.
+  symmetry in HeqR3.
+  eapply simulation__extractGenericValue in HeqR3; eauto.
+  destruct HeqR3 as [gv' [J3 J4]].
+  rewrite J3.
+  exists gv'. split; auto.
 
-      remember (_const2GV TD Mem1 gl c) as R3.
-      destruct R3 as [[gv3 t3]|]; inv H3.
-      remember (_const2GV TD Mem1 gl c0) as R4.
-      destruct R4 as [[gv4 t4]|]; inv H5.
-      erewrite H; eauto.
-      erewrite H0; eauto.
-      simpl. auto.
+  remember (_const2GV TD Mem1 gl c) as R.
+  destruct R as [[gv1 t1]|]; inv H3.
+  remember (_const2GV TD Mem1 gl c0) as R2.
+  destruct R2 as [[gv2 t2]|]; inv H5.
+  remember (Constant.getTyp c0) as R1.
+  destruct R1; inv H4.       
+  remember (insertGenericValue TD t1 gv1 l0 t2 gv2) as R3.
+  destruct R3; inv H5.   
+  symmetry in HeqR. 
+  eapply H in HeqR; eauto.
+  destruct HeqR as [gv1' [J1 J2]].
+  rewrite J1.
+  symmetry in HeqR2. 
+  eapply H0 in HeqR2; eauto.
+  destruct HeqR2 as [gv2' [J3 J4]].
+  rewrite J3.
+  symmetry in HeqR3.
+  eapply simulation__insertGenericValue in HeqR3; eauto.
+  destruct HeqR3 as [gv' [J5 J6]].
+  rewrite J5.
+  exists gv'. split; auto.
 
-      remember (_const2GV TD Mem1 gl c) as R3.
-      destruct R3 as [[gv3 t3]|]; inv H2.
-      remember (_const2GV TD Mem1 gl c0) as R4.
-      destruct R4 as [[gv4 t4]|]; inv H4.
-        erewrite H; eauto.
-        erewrite H0; eauto.
-        simpl. auto.
+  remember (_const2GV TD Mem1 gl c) as R3.
+  destruct R3 as [[gv3 t3]|]; inv H2.
+  destruct t3; inv H4.
+  remember (_const2GV TD Mem1 gl c0) as R4.
+  destruct R4 as [[gv4 t4]|]; inv H3.
+  symmetry in HeqR3. 
+  eapply H in HeqR3; eauto.
+  destruct HeqR3 as [gv3' [J3 J4]].
+  rewrite J3.
+  symmetry in HeqR4. 
+  eapply H0 in HeqR4; eauto.
+  destruct HeqR4 as [gv4' [J5 J6]].
+  rewrite J5.
+  remember (mbop TD b s gv3 gv4) as R1.
+  destruct R1; inv H4.
+  symmetry in HeqR1.
+  eapply simulation__mbop in HeqR1; eauto.
+  destruct HeqR1 as [gv' [J7 J8]].
+  rewrite J7.
+  exists gv'. split; auto.
 
-        destruct t3; inv H3.
+  remember (_const2GV TD Mem1 gl c) as R3.
+  destruct R3 as [[gv3 t3]|]; inv H2.
+  destruct t3; inv H4.
+  remember (_const2GV TD Mem1 gl c0) as R4.
+  destruct R4 as [[gv4 t4]|]; inv H3.
+  symmetry in HeqR3. 
+  eapply H in HeqR3; eauto.
+  destruct HeqR3 as [gv3' [J3 J4]].
+  rewrite J3.
+  symmetry in HeqR4. 
+  eapply H0 in HeqR4; eauto.
+  destruct HeqR4 as [gv4' [J5 J6]].
+  rewrite J5.
+  remember (mfbop TD f f0 gv3 gv4) as R1.
+  destruct R1; inv H4.
+  symmetry in HeqR1.
+  eapply simulation__mfbop in HeqR1; eauto.
+  destruct HeqR1 as [gv' [J7 J8]].
+  rewrite J7.
+  exists gv'. split; auto.
 
-      remember (_const2GV TD Mem1 gl c) as R3.
-      destruct R3 as [[gv3 t3]|]; inv H2.
-      remember (_const2GV TD Mem1 gl c0) as R4.
-      destruct R4 as [[gv4 t4]|]; inv H4.
-        erewrite H; eauto.
-        erewrite H0; eauto.
-        simpl. auto.
-
-        destruct t3; inv H3.
+  split.
+    intros gv t J.
+    inv J.
+    exists nil. unfold gv_inject. simpl. split; auto.
+ 
+    intros gv t a J.
+    inv J.
+    exists nil. unfold gv_inject. simpl. split; auto.  
 
   assert (H1':=H1).
   apply H0 with (TD:=TD)(gl:=gl) in H1'.
@@ -852,32 +1217,72 @@ Proof.
     destruct R3 as [[gv3 t3]|]; inv H2.
     remember (_const2GV TD Mem1 gl c) as R4.
     destruct R4 as [[gv4 t4]|]; inv H4.
-    erewrite H; eauto.
-    erewrite H10; eauto.
-    simpl. auto.
+    symmetry in HeqR4.
+    eapply H in HeqR4; eauto.
+    destruct HeqR4 as [gv4' [J1 J2]].
+    rewrite J1.
+    destruct (@H10 gv3 t3) as [gv3' [J3 J4]]; auto.
+    rewrite J3.
+    destruct (getTypeAllocSize TD t4); inv H3.
+    exists ((gv3' ++ gv4') ++ uninits (s - sizeGenericValue gv4')).
+    erewrite <- gv_inject__eq__sizeGenericValue; eauto.
+    split; auto.    
+      apply gv_inject_app.
+        apply gv_inject_app; auto.
+          unfold uninits, gv_inject. simpl. auto.
 
     remember (_list_const_struct2GV TD Mem1 gl l0) as R3.
     destruct R3 as [[[gv3 t3] a3]|]; inv H2.
     remember (_const2GV TD Mem1 gl c) as R4.
     destruct R4 as [[gv4 t4]|]; inv H4.
-    erewrite H; eauto.
-    erewrite H11; eauto.
-    simpl. auto.
+    symmetry in HeqR4.
+    eapply H in HeqR4; eauto.
+    destruct HeqR4 as [gv4' [J1 J2]].
+    rewrite J1.
+    symmetry in HeqR3.
+    destruct (@H11 gv3 t3 a3) as [gv3' [J3 J4]]; auto.
+    rewrite J3.
+    destruct (getABITypeAlignment TD t4); inv H3.
+    destruct (getTypeAllocSize TD t4); inv H4.
+    exists (gv3' ++
+            [(Vundef, AST.Mint ((n - sizeGenericValue gv4') * 8 - 1))]
+            ++ gv4' ++ uninits (s - sizeGenericValue gv4')).
+    erewrite <- gv_inject__eq__sizeGenericValue; eauto.
+    destruct (le_lt_dec n (Align.to_nat a3)); inv H3.
+      simpl_env.
+      split; auto.
+        apply gv_inject_app; auto.
+         apply gv_inject_app; auto.
+            unfold gv_inject. simpl. auto.
+         apply gv_inject_app; auto.
+            unfold uninits, gv_inject. simpl. auto.
+
+      simpl_env.
+      split; auto.
+        apply gv_inject_app; auto.
+         apply gv_inject_app; auto.
+            unfold gv_inject. simpl. auto.
+         apply gv_inject_app; auto.
+            unfold uninits, gv_inject. simpl. auto.
 Qed.
 
-Lemma sb_mem_inj___const2GV : forall Mem1 Mem2 TD gl c gv,
-  sb_mem_inj Mem1 Mem2 ->
-  _const2GV TD Mem1 gl c = Some gv ->
-  _const2GV TD Mem2 gl c = Some gv.
+Lemma sb_mem_inj___const2GV : forall mi Mem1 Mem2 TD gl c gv t,
+  Mem.mem_inj mi Mem1 Mem2 ->
+  _const2GV TD Mem1 gl c = Some (gv,t) ->
+  exists gv',
+    _const2GV TD Mem2 gl c = Some (gv',t) /\
+    gv_inject mi gv gv'.
 Proof.
   destruct sb_mem_inj__const2GV_mutrec as [J _].
   unfold sb_mem_inj__const2GV_prop in J. eauto.
 Qed.
 
-Lemma sb_mem_inj__const2GV : forall Mem Mem' TD gl c gv,
-  sb_mem_inj Mem Mem' ->
+Lemma sb_mem_inj__const2GV : forall mi Mem Mem' TD gl c gv,
+  Mem.mem_inj mi Mem Mem' ->
   const2GV TD Mem gl c = Some gv ->
-  const2GV TD Mem' gl c = Some gv.
+  exists gv',
+    const2GV TD Mem' gl c = Some gv' /\
+    gv_inject mi gv gv'.
 Proof.
   intros.
   unfold const2GV in *.
@@ -886,50 +1291,87 @@ Proof.
   destruct p.
   inv H0.
   symmetry in HeqR.
-  erewrite sb_mem_inj___const2GV; eauto.
-  simpl. auto.
+  eapply sb_mem_inj___const2GV in HeqR; eauto.
+  destruct HeqR as [gv' [J1 J2]].
+  exists gv'. rewrite J1. auto.
 Qed.
 
-Lemma simulation__getOperandValue : forall rm rm2 lc lc2 TD MM Mem Mem2 gl v gv,
-  reg_simulation rm rm2 lc lc2 ->
-  mem_simulation TD MM Mem Mem2 ->
+Lemma simulation__getOperandValue : forall mi rm rm2 lc lc2 TD MM Mem Mem2 gl v 
+                                           gv,
+  reg_simulation mi rm rm2 lc lc2 ->
+  mem_simulation mi TD MM Mem Mem2 ->
   getOperandValue TD Mem v lc gl = ret gv ->
-  getOperandValue TD Mem2 v lc2 gl = ret gv.
+  exists gv', 
+    getOperandValue TD Mem2 v lc2 gl = ret gv' /\
+    gv_inject mi gv gv'.
 Proof.
-  intros rm rm2 lc lc2 TD MM Mem Mem2 gl v gv H1 H2 H3.
+  intros mi rm rm2 lc lc2 TD MM Mem Mem2 gl v gv H1 H2 H3.
   unfold getOperandValue in *.
   destruct v.
-    destruct H1 as [H1 _]; eauto.
+    destruct H1 as [H1 _]; auto.
 
     destruct H2 as [H2 _].
     eapply sb_mem_inj__const2GV; eauto.
 Qed.
 
-Lemma simulation__BOP : forall rm rm2 lc lc2 TD MM Mem Mem2 gl bop0 sz0 v1 v2 
+Lemma simulation__BOP : forall mi rm rm2 lc lc2 TD MM Mem Mem2 gl bop0 sz0 v1 v2 
                         gv3,
-  reg_simulation rm rm2 lc lc2 ->
-  mem_simulation TD MM Mem Mem2 ->
+  reg_simulation mi rm rm2 lc lc2 ->
+  mem_simulation mi TD MM Mem Mem2 ->
   BOP TD Mem lc gl bop0 sz0 v1 v2 = ret gv3 ->
-  BOP TD Mem2 lc2 gl bop0 sz0 v1 v2 = ret gv3.
-Proof.
-  intros rm rm2 lc lc2 TD MM Mem Mem2 gl bop0 sz0 v1 v2 gv3 H1 H2 H3.
+  exists gv3',
+    BOP TD Mem2 lc2 gl bop0 sz0 v1 v2 = ret gv3' /\
+    gv_inject mi gv3 gv3'.
+Proof.  
+  intros mi rm rm2 lc lc2 TD MM Mem Mem2 gl bop0 sz0 v1 v2 gv3 H1 H2 H3.
   unfold BOP in *.
   remember (getOperandValue TD Mem v1 lc gl) as R1.
   destruct R1; inv H3.
   remember (getOperandValue TD Mem v2 lc gl) as R2.
   destruct R2; inv H0.
-  erewrite simulation__getOperandValue; eauto.
-  erewrite simulation__getOperandValue; eauto.
+  symmetry in HeqR1.
+  eapply simulation__getOperandValue in HeqR1; eauto.
+  destruct HeqR1 as [g' [J1 J2]].
+  rewrite J1.
+  symmetry in HeqR2.
+  eapply simulation__getOperandValue in HeqR2; eauto.
+  destruct HeqR2 as [g0' [J3 J4]].
+  rewrite J3.
+  eapply simulation__mbop in H3; eauto.
 Qed.
 
-Lemma mem_simulation__malloc : forall TD MM Mem Mem2 tsz gn align0 Mem' mb,
-  mem_simulation TD MM Mem Mem2 ->
-  malloc TD Mem tsz gn align0 = ret (Mem', mb) ->
-  exists Mem2', exists mb',
-    malloc TD Mem2 tsz gn align0 = ret (Mem2', mb') /\
-    mem_simulation TD MM Mem' Mem2'.
+Lemma alloc_getOperandValue_inv : forall Mem2 lo hi Mem2' mb2 TD v lc2 gl b2 i2,
+  Mem.alloc Mem2 lo hi = (Mem2', mb2) ->
+  getOperandValue TD Mem2' v lc2 gl = ret ptr2GV TD (Vptr b2 i2) ->
+  (getOperandValue TD Mem2 v lc2 gl = ret ptr2GV TD (Vptr b2 i2) /\ mb2 <> b2)
+    \/ b2 = mb2.
+Admitted. 
+
+Lemma gv_inject_incr:
+  forall f1 f2 v v',
+  inject_incr f1 f2 ->
+  gv_inject f1 v v' ->
+  gv_inject f2 v v'.
 Proof.
-  intros TD MM Mem Mem2 tsz gn align0 Mem' mb Hmsim Halloc.
+  intros. 
+  unfold gv_inject in *.
+  destruct (split v).
+  destruct (split v').
+  destruct H0.
+  split; eauto using val_list_inject_incr.
+Qed.
+
+Lemma mem_simulation__malloc : forall mi TD MM Mem Mem2 tsz gn align0 Mem' mb,
+  mem_simulation mi TD MM Mem Mem2 ->
+  malloc TD Mem tsz gn align0 = ret (Mem', mb) ->
+  exists mi', exists Mem2', exists mb',
+    malloc TD Mem2 tsz gn align0 = ret (Mem2', mb') /\
+    mem_simulation mi' TD MM Mem' Mem2' /\
+    Values.inject_incr mi mi' /\
+    mi' mb = Some (mb', 0) /\
+    (forall b, b <> mb -> mi b = mi' b).
+Proof.
+  intros mi TD MM Mem Mem2 tsz gn align0 Mem' mb Hmsim Halloc.
   destruct Hmsim as [H1 [H2 H3]].
   unfold malloc in *.
   remember (GV2int TD Size.ThirtyTwo gn) as R.
@@ -939,59 +1381,220 @@ Proof.
   inv Halloc.
   remember (Mem.alloc Mem2 0 (Size.to_Z tsz * z)) as R2.
   destruct R2 as [Mem2' mb2].
+  exists (fun b => if zeq b mb then Some (mb2,0%Z) else mi b).
   exists Mem2'. exists mb2.
   split; auto.
-  split.
-    clear H2 H3.
-
-unfold sb_mem_inj in *.
-unfold sb_meminj in *.
-
-Admitted.
-
-Lemma mem_simulation__free : forall TD MM Mem Mem2 mptr0 Mem',
-  mem_simulation TD MM Mem Mem2 ->
-  free TD Mem mptr0 = ret Mem' ->
-  exists Mem2',
-    free TD Mem2 mptr0 = ret Mem2' /\
-    mem_simulation TD MM Mem' Mem2'.
-Admitted.
-
-Lemma trans_cmd__is__correct : forall c TD lc1 rm1 als gl Mem1 MM1 lc1' als' 
-    Mem1' MM1' tr lc2 Mem2 rm2 rm1' cs ex_ids tmps ex_ids' tmps' r
-    optaddrb optaddre optaddrb' optaddre',  
-  non_temporal_cmd c ->
-  getCmdID c `notin` codom rm2 ->
-  trans_cmd ex_ids tmps optaddrb optaddre rm2 c = 
-    Some (ex_ids', tmps', cs, optaddrb', optaddre') ->
-  reg_simulation rm1 rm2 lc1 lc2 ->
-  mem_simulation TD MM1 Mem1 Mem2 ->
-  SoftBound.dbCmd TD gl lc1 rm1 als Mem1 MM1 c lc1' rm1' als' Mem1' MM1' tr r ->
-  exists lc2', exists Mem2',
-   SimpleSE.dbCmds TD gl lc2 als Mem2 cs lc2' als' Mem2' tr /\
-   reg_simulation rm1' rm2 lc1' lc2' /\
-   mem_simulation TD MM1' Mem1' Mem2'.
-Proof.
-  intros c TD lc1 rm1 als gl Mem1 MM1 lc1' als' Mem1' MM1' tr lc2 Mem2 rm2 rm1' 
-    cs ex_ids tmps ex_ids' tmps' r optaddrb optaddre optaddrb' optaddre' 
-    Hnontemp Hnotin Htrans Hrsim Hmsim HdbCmd.
-  (sb_dbCmd_cases (destruct HdbCmd) Case); simpl in Htrans;
-    try solve [inversion Hnontemp].
-
-Case "dbBop".
-  inv Htrans.
-  exists (updateAddAL GenericValue lc2 id0 gv3). exists Mem2. 
-  split.
-   assert (trace_nil = trace_app trace_nil trace_nil) as EQ. auto.
-   rewrite EQ.
-   eapply SimpleSE.dbCmds_cons; eauto.
-     apply SimpleSE.dbBop; eauto using simulation__BOP.
+  assert (inject_incr mi (fun b : Z => if zeq b mb then ret (mb2, 0) else mi b))
+    as Hinject_incr.
+    unfold inject_incr.
+    intros b b' d H.
+    destruct (zeq b mb); subst; auto.
+      admit. (* mi mb must be None. *)
   split; auto.
-    apply reg_simulation__updateAddAL; auto.
+  Case "msim".
+    split.    
+    SCase "msim1".
+      clear H2 H3.
+      destruct H1.
+      apply Mem.mk_mem_inj.
+      SSCase "mi_access".
+        intros b1 b2 d c ofs p J1 J2.
+        destruct (zeq b1 mb); subst; inv J1.
+        SSSCase "b1=mb".
+          symmetry in HeqR1.
+          symmetry in HeqR2.
+          destruct J2 as [J21 J22].
+          assert (0 <= ofs /\ ofs + size_chunk c <= Size.to_Z tsz * z) as EQ.
+            destruct (Z_le_dec 0 ofs).
+              destruct (Z_le_dec (ofs + size_chunk c) (Size.to_Z tsz * z)); auto.
+                apply Mem.perm_alloc_3 with (ofs:=ofs+size_chunk c-1) (p:=p) in 
+                  HeqR1; auto with zarith.
+                unfold Mem.range_perm in J21.
+                assert (ofs <= ofs + size_chunk c - 1 < ofs + size_chunk c) as J.
+                  assert (J':=@Memdata.size_chunk_pos c).
+                  auto with zarith.
+                apply J21 in J.           
+                contradict J; auto. 
+              apply Mem.perm_alloc_3 with (ofs:=ofs) (p:=p) in HeqR1; 
+                auto with zarith.
+              unfold Mem.range_perm in J21.
+              assert (ofs <= ofs < ofs + size_chunk c) as J.
+                assert (J':=@Memdata.size_chunk_pos c).
+                auto with zarith.
+              apply J21 in J.           
+              contradict J; auto. 
 
-admit. admit. admit.
+          apply Mem.valid_access_alloc_same with (chunk:=c)(ofs:=ofs+0) in HeqR2;
+            auto with zarith.
+            eapply Mem.valid_access_implies; eauto using perm_F_any.
 
-Case "dbMalloc".
+        SSSCase "b1<>mb".
+          eapply Mem.valid_access_alloc_other; eauto.
+          eapply Mem.valid_access_alloc_inv with (b:=mb)(lo:=0)
+            (hi:=Size.to_Z tsz * z)(p:=p) in J2; eauto.
+          destruct (eq_block); subst; try solve [eauto | contradict n; auto].
+
+      SSCase "mi_memval".
+Transparent Mem.alloc.
+        intros b1 ofs b2 d J1 J2.
+        injection HeqR1. intros NEXT MEM.
+        injection HeqR2. intros NEXT2 MEM2.
+        destruct Mem2. destruct Mem2'. destruct Mem. destruct Mem'. 
+        inv MEM.
+        inv MEM2. clear HeqR1 HeqR2.
+        simpl in *.
+        unfold Mem.perm in *. simpl in *.
+        clear maxaddress_pos0 conversion_props0 maxaddress_pos2 
+              conversion_props2.
+        unfold update.     
+        destruct (zeq b1 nextblock1); subst; inv J1.
+        SSSCase "b1=nextblock1".
+          destruct (zeq b2 b2) as [e | n]; 
+            try solve [contradict n; auto].
+          apply memval_inject_undef.
+
+        SSSCase "b1<>mb".
+          destruct (zeq b2 nextblock); subst.
+            admit. (* mi b1 cannot be Some nextblock if b1 <> nextblock1 *)
+
+            apply Memdata.memval_inject_incr with (f:=mi); auto.
+              apply mi_memval; auto.
+                clear - J2 n.
+                unfold update in J2.
+                destruct (zeq b1 nextblock1); subst; 
+                  try solve [auto | contradict n; auto].
+
+Global Opaque Mem.alloc.
+
+    split.    
+    SCase "msim2".
+      clear H1 H3.
+      intros lc2 gl b1 i1 bgv egv als addrb0 addre0 bid0 eid0 v b2 i2 J1 J2 J3.
+      eapply alloc_getOperandValue_inv in J3; eauto.
+      destruct J3 as [[J31 J32] | J3]; subst.
+      SSCase "mb2 <> b2".
+        assert (val_inject mi (Vptr b1 i1) (Vptr b2 i2)) as J.
+          inversion J2; subst.
+          destruct (zeq b1 mb); subst; eauto.
+            inv H3. contradict J32; auto.
+        destruct (@H2 lc2 gl b1 i1 bgv egv als addrb0 addre0 bid0 eid0 v b2 i2
+          J1 J J31) as 
+          [bgv' [egv' [lc2' [Mem21 [J37 [J33 [J34 [J35 [J36 J38]]]]]]]]].
+        clear H2.
+        assert (exists Mem21', 
+          dbCmds TD gl lc2 als Mem2'
+             (insn_call fake_id true false typ_void get_mmetadata_fn
+                ((p8, v)
+                 :: (p8, value_id addrb0) :: (p8, value_id addre0) :: nil)
+              :: insn_load bid0 p8 (value_id addrb0) Align.Zero
+                 :: insn_load eid0 p8 (value_id addre0) Align.Zero :: nil)
+             lc2' als Mem21' trace_nil) as J'.
+          admit. (* get_mmetadata_fn's axiom *)
+        destruct J' as [Mem21' J'].
+        exists bgv'. exists egv'. exists lc2'. exists Mem21'.
+        split; auto.
+        split; auto.
+        split; auto.
+        split; eauto using gv_inject_incr.
+        split; eauto using gv_inject_incr.
+          clear - J' J37 J38 HeqR2.
+          admit. (* ?! *) 
+
+      SSCase "mb2 = b2".
+        inversion J2; subst.
+        destruct (zeq b1 mb); subst.
+          admit . (* wf MM should map mb i1 to None. *)
+          admit.  (* wf mi should not map b1 (<>mb) to mb2 *)
+
+    SCase "msim3".
+      admit.
+
+  split; auto.
+  split.
+    destruct (zeq mb mb); auto.
+      contradict n; auto.
+
+    intros.
+    destruct (zeq b mb); subst; auto.
+      contradict H; auto.
+Qed.
+
+Lemma malloc_getOperandValue_inv2 : 
+  forall Mem2 tsz gn a0 Mem2' TD v lc2 gl gv mb2,
+  malloc TD Mem2 tsz gn a0 = Some (Mem2', mb2) ->
+  getOperandValue TD Mem2 v lc2 gl = Some gv ->
+  getOperandValue TD Mem2' v lc2 gl = Some gv.
+Admitted. 
+
+Lemma simulation__eq__GV2int : forall mi gn gn' TD,
+  gv_inject mi gn gn' ->
+  GV2int TD Size.ThirtyTwo gn = GV2int TD Size.ThirtyTwo gn'.
+Admitted.
+
+Lemma simulation__mload : forall mi TD MM Mem0 Mem2 gvp align0 gv t gvp2,
+  mem_simulation mi TD MM Mem0 Mem2 ->
+  mload TD Mem0 gvp t align0 = ret gv ->
+  gv_inject mi gvp gvp2 ->
+  exists gv2, mload TD Mem2 gvp2 t align0 = ret gv2 /\ gv_inject mi gv gv2.
+Admitted.
+
+Lemma trans_cmd__is__correct__dbMalloc : forall 
+  (lc2 : GVMap)
+  (Mem2 : mem)
+  (rm2 : rmap)
+  (cs : cmds)
+  (ex_ids : ids)
+  (tmps : ids)
+  (ex_ids' : ids)
+  (tmps' : ids)
+  (optaddrb : monad id)
+  (optaddre : monad id)
+  (optaddrb' : monad id)
+  (optaddre' : monad id)
+  (mi : meminj)
+  (id0 : atom)
+  (t : typ)
+  (v : value)
+  (align0 : align)
+  (Hnontemp : non_temporal_cmd (insn_malloc id0 t v align0))
+  (Hnotin : getCmdID (insn_malloc id0 t v align0) `notin` codom rm2)
+  (Htrans : trans_cmd ex_ids tmps optaddrb optaddre rm2
+             (insn_malloc id0 t v align0) =
+           ret (ex_ids', tmps', cs, optaddrb', optaddre'))
+  (rm : AssocList SoftBound.metadata)
+  (lc : GVMap)
+  (Hrsim : reg_simulation mi rm rm2 lc lc2)
+  (TD : TargetData)
+  (Mem0 : mem)
+  (MM : SoftBound.mmetadata)
+  (Hmsim : mem_simulation mi TD MM Mem0 Mem2)
+  (gl : GVMap)
+  (gn : GenericValue)
+  (als : list mblock)
+  (Mem' : mem)
+  (tsz : sz)
+  (mb : mblock)
+  (lc' : GVMap)
+  (rm' : SoftBound.rmetadata)
+  (n : Z)
+  (H : getTypeAllocSize TD t = ret tsz)
+  (H0 : getOperandValue TD Mem0 v lc gl = ret gn)
+  (H1 : malloc TD Mem0 tsz gn align0 = ret (Mem', mb))
+  (H2 : GV2int TD Size.ThirtyTwo gn = ret n)
+  (H3 : SoftBound.prop_reg_metadata lc rm id0 (blk2GV TD mb)
+         {|
+         SoftBound.md_base := SoftBound.base2GV TD mb;
+         SoftBound.md_bound := SoftBound.bound2GV TD mb tsz n |} = 
+       (lc', rm')),
+   exists lc2' : GVMap,
+     exists Mem2' : mem,
+       exists mi' : meminj,
+         dbCmds TD gl lc2 als Mem2 cs lc2' als Mem2' trace_nil /\
+         reg_simulation mi' rm' rm2 lc' lc2' /\
+         mem_simulation mi' TD MM Mem' Mem2' /\ inject_incr mi mi'.
+Proof.
+  intros.
+  simpl in Htrans.
   remember (lookupAL (id * id) rm2 id0) as R1.
   destruct R1; try solve [inversion Htrans].
   destruct p as [bid eid].
@@ -999,8 +1602,8 @@ Case "dbMalloc".
   destruct R2 as [tmp ex_ids''].
   inv Htrans.
   invert_prop_reg_metadata.
-  apply mem_simulation__malloc with (MM:=MM)(Mem2:=Mem2) in H1; auto.
-  destruct H1 as [Mem2' [mb' [H11 H12]]].
+  apply mem_simulation__malloc with (MM:=MM)(Mem2:=Mem2)(mi:=mi) in H1; auto.
+  destruct H1 as [mi' [Mem2' [mb' [H11 [H12 [H13 [H14 H15]]]]]]].
   exists 
     (updateAddAL _ 
       (updateAddAL _ 
@@ -1009,15 +1612,18 @@ Case "dbMalloc".
           bid (SoftBound.base2GV TD mb'))
         tmp (SoftBound.bound2GV TD mb' tsz n))
       eid (SoftBound.bound2GV TD mb' tsz n)).
-  exists Mem2'.
+  exists Mem2'. exists mi'.
   split.
+  SCase "dbCmds".
     assert (trace_nil = trace_app trace_nil trace_nil) as EQ. auto.
     rewrite EQ.
     apply SimpleSE.dbCmds_cons with 
       (lc2:=updateAddAL GenericValue lc2 id0 (blk2GV TD mb'))(als2:=als)
       (Mem2:=Mem2'); auto.
-      apply SimpleSE.dbMalloc with (gn:=gn)(tsz:=tsz); 
-        eauto using simulation__getOperandValue.
+      eapply simulation__getOperandValue in H0; eauto.
+      destruct H0 as [gn' [H00 H01]].
+      unfold malloc in H11.
+      erewrite simulation__eq__GV2int in H11; eauto.
     rewrite EQ.
     apply SimpleSE.dbCmds_cons with 
       (lc2:=updateAddAL _
@@ -1027,7 +1633,9 @@ Case "dbMalloc".
       (als2:=als)
       (Mem2:=Mem2'); auto.
       apply SimpleSE.dbCast; auto.
-        admit.
+        unfold CAST. simpl.
+        rewrite lookupAL_updateAddAL_eq.
+        auto.
     rewrite EQ.
     apply SimpleSE.dbCmds_cons with 
       (lc2:=updateAddAL _
@@ -1038,8 +1646,50 @@ Case "dbMalloc".
       )
       (als2:=als)
       (Mem2:=Mem2'); auto.
-      apply SimpleSE.dbGEP with (mp:=blk2GV TD mb')(vidxs:=[gn]); auto.
-        admit. admit. admit.
+
+      assert (exists gn', getOperandValue TD Mem2' v lc2 gl = ret gn' /\
+                          gv_inject mi gn gn') as H4.
+        eapply simulation__getOperandValue with (MM:=MM)(Mem2:=Mem2) in H0
+          ; eauto.
+        destruct H0 as [gv' [H00 H01]].
+        apply malloc_getOperandValue_inv2 with (tsz:=tsz)(gn:=gn)(a0:=align0)
+         (Mem2':=Mem2')(mb2:=mb') in H00; auto.
+        exists gv'. auto.
+      destruct H4 as [gn' [H41 H42]].
+      apply SimpleSE.dbGEP with (mp:=blk2GV TD mb')(vidxs:=[gn']); auto.
+        simpl.
+        rewrite <- lookupAL_updateAddAL_neq.
+          rewrite lookupAL_updateAddAL_eq; auto.
+          admit. (*id0 <> bid*)
+
+        simpl.
+        assert(getOperandValue TD Mem2' v
+          (updateAddAL _ (updateAddAL _ lc2 id0 (blk2GV TD mb'))
+          bid (SoftBound.base2GV TD mb')) gl = 
+          getOperandValue TD Mem2' v lc2 gl) as EQ'.
+          admit. (* id0 and bid are not in v *)
+        rewrite EQ'. clear EQ'.
+        rewrite H41. auto.
+
+        unfold SoftBound.bound2GV, GEP, blk2GV, GV2ptr, ptr2GV, val2GV.
+        simpl.
+        erewrite simulation__eq__GV2int in H2; eauto.
+        rewrite H2.
+        unfold mgetoffset. destruct TD.
+        unfold typ2utyp. simpl.
+        assert (exists ut, typ2utyp_aux (gen_utyp_maps (rev n0)) t = Some ut)
+          as H5.       
+          admit. (* wft *)
+        destruct H5 as [ut H5]. 
+        rewrite H5. simpl.
+        assert (getTypeAllocSize (l0, n0) t = 
+          getTypeAllocSize (l0, n0) (utyp2typ ut)) as H6.
+          admit. (* ?! *)
+        rewrite <- H6.
+        rewrite H. simpl.
+        rewrite Int.add_commut.
+        rewrite Int.add_zero. auto.
+
     rewrite EQ.
     apply SimpleSE.dbCmds_cons with 
       (lc2:=updateAddAL _
@@ -1053,10 +1703,392 @@ Case "dbMalloc".
       (als2:=als)
       (Mem2:=Mem2'); auto.
       apply SimpleSE.dbCast; auto.
-        admit.
+        unfold CAST. simpl.
+        rewrite lookupAL_updateAddAL_eq; auto.
 
   split; auto.
-    admit.
+  SCase "rsim".
+    clear - Hrsim H13 H14 H15 subcase.
+    split.
+      intros i0 gv1 J.
+      destruct (id_dec id0 i0); subst.
+      SSCase "id0 = i0".
+        rewrite lookupAL_updateAddAL_eq in J.
+        inv J.
+        exists (blk2GV TD mb').
+        split.
+          admit. (* i0 <> bid eid tmp *)
+ 
+          unfold gv_inject, blk2GV, ptr2GV, val2GV.
+          simpl.
+          split; eauto.
+           
+      SSCase "id0 <> i0".
+        rewrite <- lookupAL_updateAddAL_neq in J; auto.
+        destruct Hrsim as [J1 _].
+        apply J1 in J.
+        destruct J as [gv2 [J J2]].
+        exists gv2.
+        split.
+          admit. (* i0 <> bid eid tmp *)
+
+          eapply gv_inject_incr; eauto.
+
+      admit. (* lets see if the proofs need this direction. *)
+Qed.
+
+Lemma trans_cmd__is__correct__dbLoad_nptr__case : forall b0 i1 TD s t
+  b b1 i0 i2,
+  ret Vptr b0 i1 = GV2ptr TD (getPointerSize TD) null ->
+  ret Vptr b1 i2 = GV2ptr TD (getPointerSize TD) null  ->
+  ret s = getTypeAllocSize TD t ->
+  zeq b b0 && zeq b0 b1 && zle (Int.signed 31 i1) (Int.signed 31 i0) &&
+  zle (Int.signed 31 i0 + Size.to_Z s) (Int.signed 31 i2) ->
+  False.
+Proof.  
+  intros.
+  simpl in *.
+  inv H. inv H0.
+  (* H2 is false since Size.to_Z s is pos. *)
+Admitted.  
+
+Lemma trans_cmd__is__correct__dbLoad_nptr : forall
+  (lc2 : GVMap)
+  (Mem2 : mem)
+  (rm2 : rmap)
+  (cs : cmds)
+  (ex_ids : ids)
+  (tmps : ids)
+  (ex_ids' : ids)
+  (tmps' : ids)
+  (optaddrb : monad id)
+  (optaddre : monad id)
+  (optaddrb' : monad id)
+  (optaddre' : monad id)
+  (mi : meminj)
+  (id0 : id)
+  (t : typ)
+  (vp : value)
+  (align0 : align)
+  (Hnontemp : non_temporal_cmd (insn_load id0 t vp align0))
+  (Hnotin : getCmdID (insn_load id0 t vp align0) `notin` codom rm2)
+  (Htrans : trans_cmd ex_ids tmps optaddrb optaddre rm2
+             (insn_load id0 t vp align0) =
+           ret (ex_ids', tmps', cs, optaddrb', optaddre'))
+  (rm : SoftBound.rmetadata)
+  (lc : GVMap)
+  (Hrsim : reg_simulation mi rm rm2 lc lc2)
+  (TD : TargetData)
+  (Mem0 : mem)
+  (MM : SoftBound.mmetadata)
+  (Hmsim : mem_simulation mi TD MM Mem0 Mem2)
+  (gl : GVMap)
+  (als : list mblock)
+  (gvp : GenericValue)
+  (md : SoftBound.metadata)
+  (gv : GenericValue)
+  (H : SoftBound.get_reg_metadata TD Mem0 gl rm vp = md)
+  (H0 : getOperandValue TD Mem0 vp lc gl = ret gvp)
+  (H1 : SoftBound.assert_mptr TD t gvp md)
+  (H2 : mload TD Mem0 gvp t align0 = ret gv)
+  (H3 : ~ isPointerTyp t),
+   exists lc2' : GVMap,
+     exists Mem2' : mem,
+       exists mi' : meminj,
+         dbCmds TD gl lc2 als Mem2 cs lc2' als Mem2' trace_nil /\
+         reg_simulation mi' rm rm2 (updateAddAL GenericValue lc id0 gv) lc2' /\
+         mem_simulation mi' TD MM Mem0 Mem2' /\ inject_incr mi mi'.
+Proof.
+  intros.
+  simpl in Htrans.
+  remember (get_reg_metadata rm2 vp) as R.
+  destruct R; try solve [inversion Htrans].
+  destruct p as [[mt bv] ev].
+  remember (mk_tmp ex_ids) as R1. 
+  destruct R1 as [ptmp ex_ids1].
+  remember (mk_tmp ex_ids1) as R2. 
+  destruct R2 as [btmp ex_ids2].
+  remember (mk_tmp ex_ids2) as R3. 
+  destruct R3 as [etmp ex_ids3].
+  remember (isPointerTypB t) as R4.
+  destruct R4.
+  SCase "t is ptr".
+    unfold isPointerTyp in H3.
+    rewrite <- HeqR4 in H3.
+    contradict H3; auto.
+
+  SCase "t isnt ptr".
+  inv Htrans.
+  assert (J:=H1).
+  unfold SoftBound.assert_mptr in J.
+  case_eq (SoftBound.get_reg_metadata TD Mem0 gl rm vp).
+  intros md_base md_bound J1.
+  rewrite J1 in J.
+
+  remember (GV2ptr TD (getPointerSize TD) gvp) as R.
+  destruct R; try solve [inversion J].
+  destruct v; try solve [inversion J].
+  remember (GV2ptr TD (getPointerSize TD) md_base) as R1.
+  destruct R1; try solve [inversion J].
+  destruct v; try solve [inversion J].
+  remember (GV2ptr TD (getPointerSize TD) md_bound) as R2.
+  destruct R2; try solve [inversion J].
+  destruct v; try solve [inversion J].
+  remember (getTypeAllocSize TD t) as R3.
+  destruct R3; try solve [inversion J].
+  eapply simulation__getOperandValue in H0; eauto.
+  destruct H0 as [gvp2 [H00 H01]].            
+  unfold SoftBound.get_reg_metadata in J1.
+  eapply simulation__mload in H2; eauto.
+  destruct H2 as [gv2 [H21 H22]].
+  destruct Hrsim as [Hrsim1 [Hrsim2 Hrsim3]].
+  destruct vp as [pid |].
+    SSCase "vp is value_id".
+    remember (lookupAL SoftBound.metadata rm pid) as R4.
+    destruct R4; subst.
+      SSSCase "pid is in rm".
+      symmetry in HeqR8.
+      assert (HeqR8':=HeqR8).
+      apply Hrsim2 in HeqR8'.      
+      destruct HeqR8' as [bid [eid [bgv2 [egv2 [J1 [J2 [J3 [J4 J5]]]]]]]].
+      exists 
+       (updateAddAL _ 
+        (updateAddAL _ 
+          (updateAddAL _ 
+           (updateAddAL GenericValue lc2 ptmp gvp2)
+           btmp bgv2)
+          etmp egv2)
+        id0 gv2).
+      exists Mem2. exists mi.
+      split.
+        SSSSCase "dbCmds".
+
+    assert (trace_nil = trace_app trace_nil trace_nil) as EQ. auto.
+    rewrite EQ.
+    apply SimpleSE.dbCmds_cons with (lc2:=updateAddAL GenericValue lc2 ptmp gvp2)
+      (als2:=als)(Mem2:=Mem2); auto.
+      apply SimpleSE.dbCast; auto.
+        unfold CAST. simpl. simpl in H00.
+        rewrite H00. auto.
+    rewrite EQ.
+    apply SimpleSE.dbCmds_cons with 
+      (lc2:=updateAddAL _ (updateAddAL _ lc2 ptmp gvp2) btmp bgv2)(als2:=als)
+      (Mem2:=Mem2); auto.
+      apply SimpleSE.dbCast; auto.
+        unfold CAST. 
+        simpl in HeqR. rewrite J1 in HeqR. inv HeqR.
+        simpl.
+        rewrite <- lookupAL_updateAddAL_neq; auto.
+          rewrite J2. auto.
+          admit. (* fresh id *)
+    rewrite EQ.
+    apply SimpleSE.dbCmds_cons with 
+      (lc2:=updateAddAL _ (updateAddAL _ (updateAddAL _ lc2 ptmp gvp2)
+              btmp bgv2) etmp egv2)
+      (als2:=als)(Mem2:=Mem2); auto.
+      apply SimpleSE.dbCast; auto.
+        unfold CAST. 
+        simpl in HeqR. rewrite J1 in HeqR. inv HeqR.
+        simpl.
+        rewrite <- lookupAL_updateAddAL_neq; auto.
+          rewrite <- lookupAL_updateAddAL_neq; auto.
+            rewrite J3. auto.
+            admit. (* fresh id *)
+          admit. (* fresh id *)
+    rewrite EQ.
+    apply SimpleSE.dbCmds_cons with 
+      (lc2:=updateAddAL _ (updateAddAL _ (updateAddAL _ lc2 ptmp gvp2) btmp bgv2)
+        etmp egv2)
+      (als2:=als)(Mem2:=Mem2); auto.
+       clear - H00 J1 J2 J3 J4 J5 J H00 H01 HeqR0 HeqR5 HeqR6.
+       admit. (* assert_mptr_fn' axiom. *)
+    rewrite EQ.
+    apply SimpleSE.dbCmds_cons with 
+      (lc2:=updateAddAL _ (updateAddAL _ (updateAddAL _ 
+        (updateAddAL _ lc2 ptmp gvp2) btmp bgv2) etmp egv2) id0 gv2)
+      (als2:=als)(Mem2:=Mem2); auto.
+      apply SimpleSE.dbLoad with (mp:=gvp2); auto.
+        simpl.
+        rewrite <- lookupAL_updateAddAL_neq; auto.
+        rewrite <- lookupAL_updateAddAL_neq; auto.
+        rewrite <- lookupAL_updateAddAL_neq; auto.
+          admit. (* fresh id *)
+          admit. (* fresh id *)
+          admit. (* fresh id *)
+
+      split; auto.
+        SSSSCase "rsim".
+
+    clear - Hrsim1 H22 subcase subsubcase subsubsubcase subsubsubsubcase.
+    split.
+          SSSSSCase "rsim1".
+      intros i0 gv1 J.
+      destruct (id_dec id0 i0); subst.
+        rewrite lookupAL_updateAddAL_eq in J.
+        inv J.
+        exists gv2.
+        split; auto.
+          admit. (* i0 <> btmp etmp ptmp *)
+ 
+        rewrite <- lookupAL_updateAddAL_neq in J; auto.
+        apply Hrsim1 in J.
+        destruct J as [gv2' [J J2]].
+        exists gv2'.
+        split; auto.
+          admit. (* i0 <> bid eid tmp *)
+
+          SSSSSCase "rsim2".
+      admit. (* lets see if the proofs need this direction. *)
+
+      SSSCase "pid isnt in rm".
+      inv J1.
+      eapply trans_cmd__is__correct__dbLoad_nptr__case in J; eauto.
+      inversion J.
+
+    SSCase "vp is value_const".
+    remember (SoftBound.get_const_metadata c) as R.
+    destruct R. 
+      destruct p as [bc ec].
+      remember (const2GV TD Mem0 gl bc) as R1.
+      remember (const2GV TD Mem0 gl ec) as R2.
+      destruct R1; simpl in J1.       
+        destruct R2; simpl in J1.
+          inv J1.
+          simpl in HeqR.
+          rewrite <- HeqR8 in HeqR.
+          remember (Constant.getTyp c) as R3.
+          destruct R3; inv HeqR.
+          symmetry in HeqR10, HeqR9.
+          assert (Hmject:=Hmsim).
+          destruct Hmject as [Hmject _].
+          apply sb_mem_inj__const2GV with (Mem':=Mem2)(mi:=mi) in HeqR10; auto.
+          apply sb_mem_inj__const2GV with (Mem':=Mem2)(mi:=mi) in HeqR9; auto.
+          destruct HeqR10 as [mb_bound' [HeqR100 HeqR101]].            
+          destruct HeqR9 as [mb_base' [HeqR90 HeqR91]].           
+          exists 
+           (updateAddAL _ 
+            (updateAddAL _ 
+             (updateAddAL _ 
+              (updateAddAL GenericValue lc2 ptmp gvp2)
+              btmp mb_base')
+             etmp mb_bound')
+            id0 gv2).
+           exists Mem2. exists mi.
+           split.
+           SSSCase "dbCmds".
+
+    assert (trace_nil = trace_app trace_nil trace_nil) as EQ. auto.
+    rewrite EQ.
+    apply SimpleSE.dbCmds_cons with (lc2:=updateAddAL GenericValue lc2 ptmp gvp2)
+      (als2:=als)(Mem2:=Mem2); auto.
+      apply SimpleSE.dbCast; auto.
+        unfold CAST. simpl. simpl in H00.
+        rewrite H00. auto.
+    rewrite EQ.
+    apply SimpleSE.dbCmds_cons with 
+      (lc2:=updateAddAL _ (updateAddAL _ lc2 ptmp gvp2) btmp mb_base')(als2:=als)
+      (Mem2:=Mem2); auto.
+      apply SimpleSE.dbCast; auto.
+        unfold CAST. simpl. rewrite HeqR90.
+        clear - HeqR8 HeqR11.
+        admit. (* given wf typ, t0 must be of ptr. *)
+    rewrite EQ.
+    apply SimpleSE.dbCmds_cons with 
+      (lc2:=updateAddAL _ (updateAddAL _ (updateAddAL _ lc2 ptmp gvp2)
+              btmp mb_base') etmp mb_bound')
+      (als2:=als)(Mem2:=Mem2); auto.
+      apply SimpleSE.dbCast; auto.
+        unfold CAST. simpl. rewrite HeqR100.
+        clear - HeqR8 HeqR11.
+        admit. (* given wf typ, t0 must be of ptr. *)
+    rewrite EQ.
+    apply SimpleSE.dbCmds_cons with 
+      (lc2:=updateAddAL _ (updateAddAL _ (updateAddAL _ lc2 ptmp gvp2) btmp 
+        mb_base') etmp mb_bound') (als2:=als)(Mem2:=Mem2); auto.
+       clear - J HeqR0 HeqR5 HeqR6 H00 H00 H01 HeqR100 HeqR101 HeqR90 HeqR91.
+       admit. (* assert_mptr_fn' axiom. *)
+    rewrite EQ.
+    apply SimpleSE.dbCmds_cons with 
+      (lc2:=updateAddAL _ (updateAddAL _ (updateAddAL _ 
+        (updateAddAL _ lc2 ptmp gvp2) btmp mb_base') etmp mb_bound') id0 gv2)
+      (als2:=als)(Mem2:=Mem2); auto.
+      apply SimpleSE.dbLoad with (mp:=gvp2); auto.
+
+           split; auto.
+        SSSCase "rsim".
+
+    clear - Hrsim1 H22 subcase subsubcase subsubsubcase.
+    split.
+          SSSSSCase "rsim1".
+      intros i0 gv1 J.
+      destruct (id_dec id0 i0); subst.
+        rewrite lookupAL_updateAddAL_eq in J.
+        inv J.
+        exists gv2.
+        split; auto.
+          admit. (* i0 <> btmp etmp ptmp *)
+ 
+        rewrite <- lookupAL_updateAddAL_neq in J; auto.        
+        apply Hrsim1 in J.
+        destruct J as [gv2' [J J2]].
+        exists gv2'.
+        split; auto.
+          admit. (* i0 <> bid eid tmp *)
+
+          SSSSSCase "rsim2".
+      admit. (* lets see if the proofs need this direction. *)
+
+          inv J1.
+          eapply trans_cmd__is__correct__dbLoad_nptr__case in J; eauto.
+          inversion J.
+
+        inv J1.
+        eapply trans_cmd__is__correct__dbLoad_nptr__case in J; eauto.
+        inversion J.
+        
+      inv J1.
+      eapply trans_cmd__is__correct__dbLoad_nptr__case in J; eauto.
+      inversion J.
+Qed.
+
+Lemma trans_cmd__is__correct : forall c TD lc1 rm1 als gl Mem1 MM1 lc1' als' 
+    Mem1' MM1' tr lc2 Mem2 rm2 rm1' cs ex_ids tmps ex_ids' tmps' r
+    optaddrb optaddre optaddrb' optaddre' mi,  
+  non_temporal_cmd c ->
+  getCmdID c `notin` codom rm2 ->
+  trans_cmd ex_ids tmps optaddrb optaddre rm2 c = 
+    Some (ex_ids', tmps', cs, optaddrb', optaddre') ->
+  reg_simulation mi rm1 rm2 lc1 lc2 ->
+  mem_simulation mi TD MM1 Mem1 Mem2 ->
+  SoftBound.dbCmd TD gl lc1 rm1 als Mem1 MM1 c lc1' rm1' als' Mem1' MM1' tr r ->
+  exists lc2', exists Mem2', exists mi',
+    SimpleSE.dbCmds TD gl lc2 als Mem2 cs lc2' als' Mem2' tr /\
+    reg_simulation mi' rm1' rm2 lc1' lc2' /\
+    mem_simulation mi' TD MM1' Mem1' Mem2' /\
+    Values.inject_incr mi mi'.
+Proof.
+  intros c TD lc1 rm1 als gl Mem1 MM1 lc1' als' Mem1' MM1' tr lc2 Mem2 rm2 rm1' 
+    cs ex_ids tmps ex_ids' tmps' r optaddrb optaddre optaddrb' optaddre' mi
+    Hnontemp Hnotin Htrans Hrsim Hmsim HdbCmd.
+  (sb_dbCmd_cases (destruct HdbCmd) Case); try solve [inversion Hnontemp].
+
+Case "dbBop".
+  inv Htrans.
+  eapply simulation__BOP in H; eauto.
+  destruct H as [gv3' [H1 H2]].
+  exists (updateAddAL GenericValue lc2 id0 gv3'). exists Mem2. exists mi.
+  split.
+   assert (trace_nil = trace_app trace_nil trace_nil) as EQ. auto.
+   rewrite EQ.
+   eapply SimpleSE.dbCmds_cons; eauto.
+     apply SimpleSE.dbBop; auto.
+  split; auto.
+    apply reg_simulation__updateAddAL; auto.
+
+admit. admit. admit.
+
+Case "dbMalloc".
+  eapply trans_cmd__is__correct__dbMalloc; eauto.
 
 Case "dbMalloc_error".
   admit.    
@@ -1068,25 +2100,10 @@ Case "dbAlloca_error".
   admit. 
 
 Case "dbLoad_nptr".
-  remember (get_reg_metadata rm2 vp) as R.
-  destruct R; try solve [inversion Htrans].
-  destruct p as [bv ev].
-  remember (mk_tmp ex_ids) as R1. 
-  destruct R1 as [ptmp ex_ids1].
-  remember (mk_tmp ex_ids1) as R2. 
-  destruct R2 as [btmp ex_ids2].
-  remember (mk_tmp ex_ids2) as R3. 
-  destruct R3 as [etmp ex_ids3].
-  remember (isPointerTypB t) as R4.
-  destruct R4.
-    unfold isPointerTyp in H3.
-    rewrite <- HeqR4 in H3.
-    contradict H3; auto.
-
-    inv Htrans.
-    admit.
+  eapply trans_cmd__is__correct__dbLoad_nptr; eauto.
 
 Case "dbLoad_ptr".
+  simpl in Htrans.
   remember (get_reg_metadata rm2 vp) as R.
   destruct R; try solve [inversion Htrans].
   destruct p as [[mt bv] ev].
@@ -1098,12 +2115,258 @@ Case "dbLoad_ptr".
   destruct R3 as [etmp ex_ids4].
   remember (isPointerTypB t) as R4.
   destruct R4.
+SCase "t is ptr".
     remember (lookupAL (id * id) rm2 id0) as R5.
     destruct R5; try solve [inversion Htrans].
     destruct p as [bid0 eid0].
-    inv Htrans.
-    admit.
+    destruct optaddrb as [addrb | ].
+      destruct optaddre as [addre | ]; inv Htrans.
 
+(* case 1 *)
+  assert (J:=H1).
+  unfold SoftBound.assert_mptr in J.
+  case_eq (SoftBound.get_reg_metadata TD Mem0 gl rm vp).
+  intros md_base md_bound J1.
+  rewrite J1 in J.
+  remember (GV2ptr TD (getPointerSize TD) gvp) as R.
+  destruct R; try solve [inversion J].
+  destruct v; try solve [inversion J].
+  remember (GV2ptr TD (getPointerSize TD) md_base) as R1.
+  destruct R1; try solve [inversion J].
+  destruct v; try solve [inversion J].
+  remember (GV2ptr TD (getPointerSize TD) md_bound) as R2.
+  destruct R2; try solve [inversion J].
+  destruct v; try solve [inversion J].
+  remember (getTypeAllocSize TD t) as R3.
+  destruct R3; try solve [inversion J].
+  eapply simulation__getOperandValue in H0; eauto.
+  destruct H0 as [gvp2 [H00 H01]].            
+  unfold SoftBound.get_reg_metadata in J1.
+  eapply simulation__mload in H2; eauto.
+  destruct H2 as [gv2 [H21 H22]].
+  destruct Hrsim as [Hrsim1 [Hrsim2 Hrsim3]].
+  case_eq (SoftBound.get_mem_metadata TD MM gvp).
+  intros mb_base0 md_bound0 JJ.
+  unfold SoftBound.get_mem_metadata in JJ.
+
+(*
+  destruct vp as [pid |].
+    SSCase "vp is value_id".
+    remember (lookupAL SoftBound.metadata rm pid) as R4.
+    destruct R4; subst.
+      SSSCase "pid is in rm".
+      symmetry in HeqR9.
+      assert (HeqR9':=HeqR9).
+      apply Hrsim2 in HeqR9'.      
+      destruct HeqR9' as [bid [eid [bgv2 [egv2 [J1 [J2 [J3 [J4 J5]]]]]]]].
+      exists 
+       (updateAddAL _ 
+        (updateAddAL _ 
+          (updateAddAL _ 
+           (updateAddAL GenericValue lc2 ptmp gvp2)
+           btmp bgv2)
+          etmp egv2)
+        id0 gv2).
+      exists Mem2. exists mi.
+      split.
+        SSSSCase "dbCmds".
+
+    assert (trace_nil = trace_app trace_nil trace_nil) as EQ. auto.
+    rewrite EQ.
+    apply SimpleSE.dbCmds_cons with (lc2:=updateAddAL GenericValue lc2 ptmp gvp2)
+      (als2:=als)(Mem2:=Mem2); auto.
+      apply SimpleSE.dbCast; auto.
+        unfold CAST. simpl. simpl in H00.
+        rewrite H00. auto.
+    rewrite EQ.
+    apply SimpleSE.dbCmds_cons with 
+      (lc2:=updateAddAL _ (updateAddAL _ lc2 ptmp gvp2) btmp bgv2)(als2:=als)
+      (Mem2:=Mem2); auto.
+      apply SimpleSE.dbCast; auto.
+        unfold CAST. 
+        simpl in HeqR. rewrite J1 in HeqR. inv HeqR.
+        simpl.
+        rewrite <- lookupAL_updateAddAL_neq; auto.
+          rewrite J2. auto.
+          admit. (* fresh id *)
+    rewrite EQ.
+    apply SimpleSE.dbCmds_cons with 
+      (lc2:=updateAddAL _ (updateAddAL _ (updateAddAL _ lc2 ptmp gvp2)
+              btmp bgv2) etmp egv2)
+      (als2:=als)(Mem2:=Mem2); auto.
+      apply SimpleSE.dbCast; auto.
+        unfold CAST. 
+        simpl in HeqR. rewrite J1 in HeqR. inv HeqR.
+        simpl.
+        rewrite <- lookupAL_updateAddAL_neq; auto.
+          rewrite <- lookupAL_updateAddAL_neq; auto.
+            rewrite J3. auto.
+            admit. (* fresh id *)
+          admit. (* fresh id *)
+    rewrite EQ.
+    apply SimpleSE.dbCmds_cons with 
+      (lc2:=updateAddAL _ (updateAddAL _ (updateAddAL _ lc2 ptmp gvp2) btmp bgv2)
+        etmp egv2)
+      (als2:=als)(Mem2:=Mem2); auto.
+       clear - H00 J1 J2 J3 J4 J5 J H00 H01 HeqR0 HeqR5 HeqR6.
+       admit. (* assert_mptr_fn' axiom. *)
+    rewrite EQ.
+    apply SimpleSE.dbCmds_cons with 
+      (lc2:=updateAddAL _ (updateAddAL _ (updateAddAL _ 
+        (updateAddAL _ lc2 ptmp gvp2) btmp bgv2) etmp egv2) id0 gv2)
+      (als2:=als)(Mem2:=Mem2); auto.
+      apply SimpleSE.dbLoad with (mp:=gvp2); auto.
+        simpl.
+        rewrite <- lookupAL_updateAddAL_neq; auto.
+        rewrite <- lookupAL_updateAddAL_neq; auto.
+        rewrite <- lookupAL_updateAddAL_neq; auto.
+          admit. (* fresh id *)
+          admit. (* fresh id *)
+          admit. (* fresh id *)
+
+      split; auto.
+        SSSSCase "rsim".
+
+    clear - Hrsim1 H22 subcase subsubcase subsubsubcase subsubsubsubcase.
+    split.
+          SSSSSCase "rsim1".
+      intros i0 gv1 J.
+      destruct (id_dec id0 i0); subst.
+        rewrite lookupAL_updateAddAL_eq in J.
+        inv J.
+        exists gv2.
+        split; auto.
+          admit. (* i0 <> btmp etmp ptmp *)
+ 
+        rewrite <- lookupAL_updateAddAL_neq in J; auto.
+        apply Hrsim1 in J.
+        destruct J as [gv2' [J J2]].
+        exists gv2'.
+        split; auto.
+          admit. (* i0 <> bid eid tmp *)
+
+          SSSSSCase "rsim2".
+      admit. (* lets see if the proofs need this direction. *)
+
+      SSSCase "pid isnt in rm".
+      inv J1.
+      eapply trans_cmd__is__correct__dbLoad_nptr__case in J; eauto.
+      inversion J.
+
+    SSCase "vp is value_const".
+    remember (SoftBound.get_const_metadata c) as R.
+    destruct R. 
+      destruct p as [bc ec].
+      remember (const2GV TD Mem0 gl bc) as R1.
+      remember (const2GV TD Mem0 gl ec) as R2.
+      destruct R1; simpl in J1.       
+        destruct R2; simpl in J1.
+          inv J1.
+          simpl in HeqR.
+          rewrite <- HeqR8 in HeqR.
+          remember (Constant.getTyp c) as R3.
+          destruct R3; inv HeqR.
+          symmetry in HeqR10, HeqR9.
+          assert (Hmject:=Hmsim).
+          destruct Hmject as [Hmject _].
+          apply sb_mem_inj__const2GV with (Mem':=Mem2)(mi:=mi) in HeqR10; auto.
+          apply sb_mem_inj__const2GV with (Mem':=Mem2)(mi:=mi) in HeqR9; auto.
+          destruct HeqR10 as [mb_bound' [HeqR100 HeqR101]].            
+          destruct HeqR9 as [mb_base' [HeqR90 HeqR91]].           
+          exists 
+           (updateAddAL _ 
+            (updateAddAL _ 
+             (updateAddAL _ 
+              (updateAddAL GenericValue lc2 ptmp gvp2)
+              btmp mb_base')
+             etmp mb_bound')
+            id0 gv2).
+           exists Mem2. exists mi.
+           split.
+           SSSCase "dbCmds".
+
+    assert (trace_nil = trace_app trace_nil trace_nil) as EQ. auto.
+    rewrite EQ.
+    apply SimpleSE.dbCmds_cons with (lc2:=updateAddAL GenericValue lc2 ptmp gvp2)
+      (als2:=als)(Mem2:=Mem2); auto.
+      apply SimpleSE.dbCast; auto.
+        unfold CAST. simpl. simpl in H00.
+        rewrite H00. auto.
+    rewrite EQ.
+    apply SimpleSE.dbCmds_cons with 
+      (lc2:=updateAddAL _ (updateAddAL _ lc2 ptmp gvp2) btmp mb_base')(als2:=als)
+      (Mem2:=Mem2); auto.
+      apply SimpleSE.dbCast; auto.
+        unfold CAST. simpl. rewrite HeqR90.
+        clear - HeqR8 HeqR11.
+        admit. (* given wf typ, t0 must be of ptr. *)
+    rewrite EQ.
+    apply SimpleSE.dbCmds_cons with 
+      (lc2:=updateAddAL _ (updateAddAL _ (updateAddAL _ lc2 ptmp gvp2)
+              btmp mb_base') etmp mb_bound')
+      (als2:=als)(Mem2:=Mem2); auto.
+      apply SimpleSE.dbCast; auto.
+        unfold CAST. simpl. rewrite HeqR100.
+        clear - HeqR8 HeqR11.
+        admit. (* given wf typ, t0 must be of ptr. *)
+    rewrite EQ.
+    apply SimpleSE.dbCmds_cons with 
+      (lc2:=updateAddAL _ (updateAddAL _ (updateAddAL _ lc2 ptmp gvp2) btmp 
+        mb_base') etmp mb_bound') (als2:=als)(Mem2:=Mem2); auto.
+       clear - J HeqR0 HeqR5 HeqR6 H00 H00 H01 HeqR100 HeqR101 HeqR90 HeqR91.
+       admit. (* assert_mptr_fn' axiom. *)
+    rewrite EQ.
+    apply SimpleSE.dbCmds_cons with 
+      (lc2:=updateAddAL _ (updateAddAL _ (updateAddAL _ 
+        (updateAddAL _ lc2 ptmp gvp2) btmp mb_base') etmp mb_bound') id0 gv2)
+      (als2:=als)(Mem2:=Mem2); auto.
+      apply SimpleSE.dbLoad with (mp:=gvp2); auto.
+
+           split; auto.
+        SSSCase "rsim".
+
+    clear - Hrsim1 H22 subcase subsubcase subsubsubcase.
+    split.
+          SSSSSCase "rsim1".
+      intros i0 gv1 J.
+      destruct (id_dec id0 i0); subst.
+        rewrite lookupAL_updateAddAL_eq in J.
+        inv J.
+        exists gv2.
+        split; auto.
+          admit. (* i0 <> btmp etmp ptmp *)
+ 
+        rewrite <- lookupAL_updateAddAL_neq in J; auto.        
+        apply Hrsim1 in J.
+        destruct J as [gv2' [J J2]].
+        exists gv2'.
+        split; auto.
+          admit. (* i0 <> bid eid tmp *)
+
+          SSSSSCase "rsim2".
+      admit. (* lets see if the proofs need this direction. *)
+
+          inv J1.
+          eapply trans_cmd__is__correct__dbLoad_nptr__case in J; eauto.
+          inversion J.
+
+        inv J1.
+        eapply trans_cmd__is__correct__dbLoad_nptr__case in J; eauto.
+        inversion J.
+        
+      inv J1.
+      eapply trans_cmd__is__correct__dbLoad_nptr__case in J; eauto.
+      inversion J.
+
+    admit.
+*)
+       admit.
+
+(* case 2 *)
+      destruct optaddre as [addre | ]; inv Htrans.
+        admit.
+
+SCase "t isnt ptr".
     unfold isPointerTyp in H3.
     rewrite <- HeqR4 in H3.
     inversion H3.
@@ -1111,6 +2374,7 @@ Case "dbLoad_ptr".
 admit. admit. admit.
 
 Case "dbLoad_abort".
+  simpl in Htrans.
   remember (get_reg_metadata rm2 vp) as R.
   destruct R; try solve [inversion Htrans].
   destruct p as [[mt bv] ev].
@@ -1132,6 +2396,7 @@ Case "dbLoad_abort".
     admit.
 
 Case "dbStore_nptr".
+  simpl in Htrans.
   remember (get_reg_metadata rm2 vp) as R.
   destruct R; try solve [inversion Htrans].
   destruct p as [[mt bv] ev].
@@ -1151,6 +2416,7 @@ Case "dbStore_nptr".
     admit.
 
 Case "dbStore_ptr".
+  simpl in Htrans.
   remember (get_reg_metadata rm2 vp) as R.
   destruct R; try solve [inversion Htrans].
   destruct p as [[mt bv] ev].
@@ -1175,6 +2441,7 @@ Case "dbStore_ptr".
 admit. admit. admit.
 
 Case "dbStore_abort".
+  simpl in Htrans.
   remember (get_reg_metadata rm2 vp) as R.
   destruct R; try solve [inversion Htrans].
   destruct p as [[mt bv] ev].
@@ -1205,19 +2472,20 @@ end.
 
 Lemma trans_cmds__is__correct : forall cs TD lc1 rm1 als gl Mem1 MM1 lc1' als' 
     Mem1' MM1' tr lc2 Mem2 rm2 rm1' cs' ex_ids tmps ex_ids' tmps' r
-    optaddrb optaddre optaddrb' optaddre', 
+    optaddrb optaddre optaddrb' optaddre' mi, 
   non_temporal_cmds cs ->
   AtomSetImpl.inter (getCmdsIDs cs) (codom rm2) [<=] empty ->
   trans_cmds ex_ids tmps optaddrb optaddre rm2 cs = 
     Some (ex_ids', tmps', cs', optaddrb', optaddre') ->
-  reg_simulation rm1 rm2 lc1 lc2 ->
-  mem_simulation TD MM1 Mem1 Mem2 ->
+  reg_simulation mi rm1 rm2 lc1 lc2 ->
+  mem_simulation mi TD MM1 Mem1 Mem2 ->
   SoftBound.dbCmds TD gl lc1 rm1 als Mem1 MM1 cs lc1' rm1' als' Mem1' MM1' tr r 
     ->
-  exists lc2', exists Mem2',
+  exists lc2', exists Mem2', exists mi',
     SimpleSE.dbCmds TD gl lc2 als Mem2 cs' lc2' als' Mem2' tr /\
-    reg_simulation rm1' rm2 lc1' lc2' /\
-    mem_simulation TD MM1' Mem1' Mem2'.
+    reg_simulation mi' rm1' rm2 lc1' lc2' /\
+    mem_simulation mi' TD MM1' Mem1' Mem2' /\
+    Values.inject_incr mi mi'.
 Admitted.
 
 End SBpass.
