src/SoftBound/sb_tactic.v
@@ -5,6 +5,7 @@ Add LoadPath "../ssa".
 Add LoadPath "../../../theory/metatheory_8.3".
 Add LoadPath "../TV".
 Require Import sb_def.
+Require Import Metatheory.
 
 Ltac invert_prop_reg_metadata :=
   match goal with
@@ -20,6 +21,10 @@ Ltac invert_result :=
   | [H : SoftBound.rok = SoftBound.rerror |- _ ] => inversion H 
   | [H : SoftBound.rok = SoftBound.rabort |- _ ] => inversion H 
  end.
+
+Ltac SSSSSCase name := Case_aux subsubsubsubsubcase name.
+Ltac SSSSSSCase name := Case_aux subsubsubsubsubsubcase name.
+Ltac SSSSSSSCase name := Case_aux subsubsubsubsubsubsubcase name.
 
 (*****************************)
 (*
